src/proofs/no_slashable_attestations/supporting_lemmas/dv_next_invs_8_18.dfy
@@ -232,7 +232,7 @@ module DV_Next_Invs_8_18
     requires inv_quorum_constraints(dv)  
     requires inv_unchanged_honesty(dv)
     requires inv4(dv)
-    requires inv5(dv)
+    requires inv_queued_att_duty_is_rcvd_duty(dv)
     requires inv_is_sequence_attestation_duties_to_be_serves_orders(dv)
     requires concl_future_att_duty_is_higher_than_queued_att_duty(dv)
     requires inv_strictly_increasing_queue_of_att_duties(dv)
@@ -295,7 +295,7 @@ module DV_Next_Invs_8_18
     requires inv_quorum_constraints(dv)  
     requires inv_unchanged_honesty(dv)  
     requires inv4(dv)
-    requires inv5(dv)
+    requires inv_queued_att_duty_is_rcvd_duty(dv)
     requires inv_latest_served_duty_is_rcvd_duty(dv)
     requires inv_is_sequence_attestation_duties_to_be_serves_orders(dv)  
     requires inv_strictly_increasing_queue_of_att_duties(dv)
@@ -324,8 +324,8 @@ module DV_Next_Invs_8_18
                        
                     case ImportedNewBlock(block) =>                     
                         var dvc_mod := add_block_to_bn(dvc, block);
-                        lemma_inv5_add_block_to_bn(dvc, block, dvc_mod);
-                        assert inv5_body(dvc_mod);
+                        lemma_inv_queued_att_duty_is_rcvd_duty_add_block_to_bn(dvc, block, dvc_mod);
+                        assert inv_queued_att_duty_is_rcvd_duty_body(dvc_mod);
                         lemma_inv_strictly_increasing_queue_of_att_duties_add_block_to_bn(dvc, block, dvc_mod);
                         assert inv_strictly_increasing_queue_of_att_duties_body(dvc_mod);
                         lemma_inv_queued_att_duty_is_higher_than_latest_served_att_duty_add_block_to_bn(dvc, block, dvc_mod);
