src/proofs/no_slashable_attestations/supporting_lemmas/fnc_invs_1_26.dfy
@@ -202,32 +202,32 @@ module Fnc_Invs_1_26
     requires s.all_rcvd_duties == s'.all_rcvd_duties
     { } 
 
-    lemma lemma_inv5_add_block_to_bn(
+    lemma lemma_inv_queued_att_duty_is_rcvd_duty_add_block_to_bn(
         s: DVCState,
         block: BeaconBlock,
         s': DVCState 
     )
     requires add_block_to_bn.requires(s, block)
     requires s' == add_block_to_bn(s, block)
-    requires inv5_body(s)
-    ensures inv5_body(s')
+    requires inv_queued_att_duty_is_rcvd_duty_body(s)
+    ensures inv_queued_att_duty_is_rcvd_duty_body(s')
     { } 
     
-    lemma lemma_inv5_f_start_next_duty(process: DVCState, attestation_duty: AttestationDuty, process': DVCState)
+    lemma lemma_inv_queued_att_duty_is_rcvd_duty_f_start_next_duty(process: DVCState, attestation_duty: AttestationDuty, process': DVCState)
     requires f_start_next_duty.requires(process, attestation_duty)
     requires process' == f_start_next_duty(process, attestation_duty).state
-    requires inv5_body(process)
-    ensures inv5_body(process')
+    requires inv_queued_att_duty_is_rcvd_duty_body(process)
+    ensures inv_queued_att_duty_is_rcvd_duty_body(process')
     { }  
 
-    lemma lemma_inv5_f_check_for_next_queued_duty(
+    lemma lemma_inv_queued_att_duty_is_rcvd_duty_f_check_for_next_queued_duty(
         process: DVCState,
         process': DVCState
     )
     requires f_check_for_next_queued_duty.requires(process)
     requires process' == f_check_for_next_queued_duty(process).state
-    requires inv5_body(process)
-    ensures inv5_body(process')
+    requires inv_queued_att_duty_is_rcvd_duty_body(process)
+    ensures inv_queued_att_duty_is_rcvd_duty_body(process')
     decreases process.attestation_duties_queue
     {
         if  && process.attestation_duties_queue != [] 
@@ -249,14 +249,14 @@ module Fnc_Invs_1_26
                             new_attestation_slashing_db
                         )                        
                     );
-                    lemma_inv5_f_check_for_next_queued_duty(process_mod, process');
+                    lemma_inv_queued_att_duty_is_rcvd_duty_f_check_for_next_queued_duty(process_mod, process');
                 }
                 else
                 { 
                     var process_mod := process.(
                         attestation_duties_queue := process.attestation_duties_queue[1..]
                     );         
-                    lemma_inv5_f_start_next_duty(process_mod, process.attestation_duties_queue[0], process');
+                    lemma_inv_queued_att_duty_is_rcvd_duty_f_start_next_duty(process_mod, process.attestation_duties_queue[0], process');
                 }
         }
         else
@@ -265,27 +265,27 @@ module Fnc_Invs_1_26
         }
     }
 
-    lemma lemma_inv5_f_serve_attestation_duty(
+    lemma lemma_inv_queued_att_duty_is_rcvd_duty_f_serve_attestation_duty(
         process: DVCState,
         attestation_duty: AttestationDuty,
         process': DVCState
     )  
     requires f_serve_attestation_duty.requires(process, attestation_duty)
     requires process' == f_serve_attestation_duty(process, attestation_duty).state
-    requires inv5_body(process)
-    ensures inv5_body(process')
+    requires inv_queued_att_duty_is_rcvd_duty_body(process)
+    ensures inv_queued_att_duty_is_rcvd_duty_body(process')
     {
         var process_mod := process.(
                 attestation_duties_queue := process.attestation_duties_queue + [attestation_duty],
                 all_rcvd_duties := process.all_rcvd_duties + {attestation_duty}
             );        
 
-        assert inv5_body(process_mod);
+        assert inv_queued_att_duty_is_rcvd_duty_body(process_mod);
 
-        lemma_inv5_f_check_for_next_queued_duty(process_mod, process');        
+        lemma_inv_queued_att_duty_is_rcvd_duty_f_check_for_next_queued_duty(process_mod, process');        
     }    
 
-    lemma lemma_inv5_f_att_consensus_decided(
+    lemma lemma_inv_queued_att_duty_is_rcvd_duty_f_att_consensus_decided(
         process: DVCState,
         id: Slot,
         decided_attestation_data: AttestationData, 
@@ -293,8 +293,8 @@ module Fnc_Invs_1_26
     )
     requires f_att_consensus_decided.requires(process, id, decided_attestation_data)
     requires process' == f_att_consensus_decided(process, id, decided_attestation_data).state 
-    requires inv5_body(process)
-    ensures inv5_body(process')
+    requires inv_queued_att_duty_is_rcvd_duty_body(process)
+    ensures inv_queued_att_duty_is_rcvd_duty_body(process')
     {
         
         if  && process.current_attestation_duty.isPresent()
@@ -323,36 +323,36 @@ module Fnc_Invs_1_26
                     )
                 );
 
-            assert inv5_body(process);
+            assert inv_queued_att_duty_is_rcvd_duty_body(process);
 
             var ret_check_for_next_queued_duty := f_check_for_next_queued_duty(process);
             
-            lemma_inv5_f_check_for_next_queued_duty(process, ret_check_for_next_queued_duty.state);
+            lemma_inv_queued_att_duty_is_rcvd_duty_f_check_for_next_queued_duty(process, ret_check_for_next_queued_duty.state);
 
             assert process' == ret_check_for_next_queued_duty.state;
         }
     }  
 
-    lemma lemma_inv5_f_listen_for_attestation_shares(
+    lemma lemma_inv_queued_att_duty_is_rcvd_duty_f_listen_for_attestation_shares(
         process: DVCState,
         attestation_share: AttestationShare,
         process': DVCState
     )
     requires f_listen_for_attestation_shares.requires(process, attestation_share)
     requires process' == f_listen_for_attestation_shares(process, attestation_share).state
-    requires inv5_body(process)
-    ensures inv5_body(process')
+    requires inv_queued_att_duty_is_rcvd_duty_body(process)
+    ensures inv_queued_att_duty_is_rcvd_duty_body(process')
     {}
 
-    lemma lemma_inv5_f_listen_for_new_imported_blocks(
+    lemma lemma_inv_queued_att_duty_is_rcvd_duty_f_listen_for_new_imported_blocks(
         process: DVCState,
         block: BeaconBlock,
         process': DVCState
     )
     requires f_listen_for_new_imported_blocks.requires(process, block)
     requires process' == f_listen_for_new_imported_blocks(process, block).state
-    requires inv5_body(process)
-    ensures inv5_body(process')
+    requires inv_queued_att_duty_is_rcvd_duty_body(process)
+    ensures inv_queued_att_duty_is_rcvd_duty_body(process')
     {
         var new_consensus_instances_already_decided := f_listen_for_new_imported_blocks_helper_1(process, block);
 
@@ -372,7 +372,7 @@ module Fnc_Invs_1_26
                     rcvd_attestation_shares := process.rcvd_attestation_shares - att_consensus_instances_already_decided.Keys                    
                 );    
 
-        assert inv5_body(process);
+        assert inv_queued_att_duty_is_rcvd_duty_body(process);
                     
 
         if process.current_attestation_duty.isPresent() && process.current_attestation_duty.safe_get().slot in att_consensus_instances_already_decided
@@ -388,13 +388,13 @@ module Fnc_Invs_1_26
                 )                
             );
 
-            assert inv5_body(process);
+            assert inv_queued_att_duty_is_rcvd_duty_body(process);
 
-            lemma_inv5_f_check_for_next_queued_duty(process, process');
+            lemma_inv_queued_att_duty_is_rcvd_duty_f_check_for_next_queued_duty(process, process');
         }
         else
         {
-            assert inv5_body(process);
+            assert inv_queued_att_duty_is_rcvd_duty_body(process);
         }
     }  
 
@@ -412,7 +412,7 @@ module Fnc_Invs_1_26
     )
     requires f_check_for_next_queued_duty.requires(process)
     requires process' == f_check_for_next_queued_duty(process).state
-    requires inv5_body(process)
+    requires inv_queued_att_duty_is_rcvd_duty_body(process)
     requires inv_current_att_duty_is_rcvd_duty_body(process)
     ensures inv_current_att_duty_is_rcvd_duty_body(process')
     decreases process.attestation_duties_queue
@@ -460,7 +460,7 @@ module Fnc_Invs_1_26
     )  
     requires f_serve_attestation_duty.requires(process, attestation_duty)
     requires process' == f_serve_attestation_duty(process, attestation_duty).state
-    requires inv5_body(process)
+    requires inv_queued_att_duty_is_rcvd_duty_body(process)
     requires inv_current_att_duty_is_rcvd_duty_body(process)
     ensures inv_current_att_duty_is_rcvd_duty_body(process')
     {
@@ -482,7 +482,7 @@ module Fnc_Invs_1_26
     )
     requires f_att_consensus_decided.requires(process, id, decided_attestation_data)
     requires process' == f_att_consensus_decided(process, id, decided_attestation_data).state 
-    requires inv5_body(process)
+    requires inv_queued_att_duty_is_rcvd_duty_body(process)
     requires inv_current_att_duty_is_rcvd_duty_body(process)
     ensures inv_current_att_duty_is_rcvd_duty_body(process')
     {
@@ -541,7 +541,7 @@ module Fnc_Invs_1_26
     )
     requires f_listen_for_new_imported_blocks.requires(process, block)
     requires process' == f_listen_for_new_imported_blocks(process, block).state
-    requires inv5_body(process)
+    requires inv_queued_att_duty_is_rcvd_duty_body(process)
     requires inv_current_att_duty_is_rcvd_duty_body(process)
     ensures inv_current_att_duty_is_rcvd_duty_body(process')
     {
@@ -579,7 +579,7 @@ module Fnc_Invs_1_26
                 )                
             );
 
-            assert inv5_body(process);
+            assert inv_queued_att_duty_is_rcvd_duty_body(process);
             assert inv_current_att_duty_is_rcvd_duty_body(process);
 
             lemma_inv_current_att_duty_is_rcvd_duty_f_check_for_next_queued_duty(process, process');
@@ -604,7 +604,7 @@ module Fnc_Invs_1_26
     )
     requires f_check_for_next_queued_duty.requires(process)
     requires process' == f_check_for_next_queued_duty(process).state
-    requires inv5_body(process)
+    requires inv_queued_att_duty_is_rcvd_duty_body(process)
     requires inv_latest_served_duty_is_rcvd_duty_body(process)
     ensures inv_latest_served_duty_is_rcvd_duty_body(process')
     decreases process.attestation_duties_queue
@@ -652,7 +652,7 @@ module Fnc_Invs_1_26
     )  
     requires f_serve_attestation_duty.requires(process, attestation_duty)
     requires process' == f_serve_attestation_duty(process, attestation_duty).state
-    requires inv5_body(process)
+    requires inv_queued_att_duty_is_rcvd_duty_body(process)
     requires inv_latest_served_duty_is_rcvd_duty_body(process)
     ensures inv_latest_served_duty_is_rcvd_duty_body(process')
     {
@@ -674,7 +674,7 @@ module Fnc_Invs_1_26
     )
     requires f_att_consensus_decided.requires(process, id, decided_attestation_data)
     requires process' == f_att_consensus_decided(process, id, decided_attestation_data).state 
-    requires inv5_body(process)
+    requires inv_queued_att_duty_is_rcvd_duty_body(process)
     requires inv_latest_served_duty_is_rcvd_duty_body(process)
     ensures inv_latest_served_duty_is_rcvd_duty_body(process')
     {
@@ -734,7 +734,7 @@ module Fnc_Invs_1_26
     )
     requires f_listen_for_new_imported_blocks.requires(process, block)
     requires process' == f_listen_for_new_imported_blocks(process, block).state
-    requires inv5_body(process)
+    requires inv_queued_att_duty_is_rcvd_duty_body(process)
     requires inv_latest_served_duty_is_rcvd_duty_body(process)
     ensures inv_latest_served_duty_is_rcvd_duty_body(process')
     {
@@ -772,7 +772,7 @@ module Fnc_Invs_1_26
                 )                
             );
 
-            assert inv5_body(process);
+            assert inv_queued_att_duty_is_rcvd_duty_body(process);
             assert inv_latest_served_duty_is_rcvd_duty_body(process);
 
             lemma_inv_latest_served_duty_is_rcvd_duty_f_check_for_next_queued_duty(process, process');
@@ -1813,7 +1813,7 @@ module Fnc_Invs_1_26
     )  
     requires f_serve_attestation_duty.requires(process, attestation_duty)
     requires process' == f_serve_attestation_duty(process, attestation_duty).state
-    requires inv5_body(process)  
+    requires inv_queued_att_duty_is_rcvd_duty_body(process)  
     requires concl_future_att_duty_is_higher_than_queued_att_duty_body(process, attestation_duty)  
     requires inv_strictly_increasing_queue_of_att_duties_body(process)
     ensures inv_strictly_increasing_queue_of_att_duties_body(process')
@@ -1833,7 +1833,7 @@ module Fnc_Invs_1_26
     )
     requires f_listen_for_attestation_shares.requires(process, attestation_share)
     requires process' == f_listen_for_attestation_shares(process, attestation_share).state    
-    requires inv5_body(process)
+    requires inv_queued_att_duty_is_rcvd_duty_body(process)
     requires inv_strictly_increasing_queue_of_att_duties_body(process)
     requires inv_queued_att_duty_is_higher_than_latest_served_att_duty_body(process)
     ensures inv_queued_att_duty_is_higher_than_latest_served_att_duty_body(process')
@@ -1844,7 +1844,7 @@ module Fnc_Invs_1_26
         process': DVCState)
     requires f_resend_attestation_share.requires(process)
     requires process' == f_resend_attestation_share(process).state    
-    requires inv5_body(process)
+    requires inv_queued_att_duty_is_rcvd_duty_body(process)
     requires inv_strictly_increasing_queue_of_att_duties_body(process)
     requires inv_queued_att_duty_is_higher_than_latest_served_att_duty_body(process)
     ensures inv_queued_att_duty_is_higher_than_latest_served_att_duty_body(process')
@@ -1857,7 +1857,7 @@ module Fnc_Invs_1_26
     )
     requires add_block_to_bn.requires(s, block)
     requires s' == add_block_to_bn(s, block)
-    requires inv5_body(s)
+    requires inv_queued_att_duty_is_rcvd_duty_body(s)
     requires inv_strictly_increasing_queue_of_att_duties_body(s)
     requires inv_queued_att_duty_is_higher_than_latest_served_att_duty_body(s)
     ensures inv_queued_att_duty_is_higher_than_latest_served_att_duty_body(s')
@@ -1868,7 +1868,7 @@ module Fnc_Invs_1_26
     requires process' == f_start_next_duty(process, attestation_duty).state   
     requires forall queued_duty: AttestationDuty | queued_duty in process.attestation_duties_queue ::
                         attestation_duty.slot < queued_duty.slot     
-    requires inv5_body(process)
+    requires inv_queued_att_duty_is_rcvd_duty_body(process)
     requires inv_strictly_increasing_queue_of_att_duties_body(process)                        
     requires inv_queued_att_duty_is_higher_than_latest_served_att_duty_body(process)
     ensures inv_queued_att_duty_is_higher_than_latest_served_att_duty_body(process')
@@ -1880,7 +1880,7 @@ module Fnc_Invs_1_26
     )
     requires f_check_for_next_queued_duty.requires(process)
     requires process' == f_check_for_next_queued_duty(process).state    
-    requires inv5_body(process)
+    requires inv_queued_att_duty_is_rcvd_duty_body(process)
     requires inv_strictly_increasing_queue_of_att_duties_body(process)
     requires inv_queued_att_duty_is_higher_than_latest_served_att_duty_body(process)
     ensures inv_strictly_increasing_queue_of_att_duties_body(process')
@@ -1938,7 +1938,7 @@ module Fnc_Invs_1_26
     )  
     requires f_serve_attestation_duty.requires(process, attestation_duty)
     requires process' == f_serve_attestation_duty(process, attestation_duty).state
-    requires inv5_body(process)  
+    requires inv_queued_att_duty_is_rcvd_duty_body(process)  
     requires concl_next_att_duty_is_higher_than_latest_served_att_duty_body(process, attestation_duty)  
     requires concl_future_att_duty_is_higher_than_queued_att_duty_body(process, attestation_duty)  
     requires inv_strictly_increasing_queue_of_att_duties_body(process)
@@ -1979,7 +1979,7 @@ module Fnc_Invs_1_26
     )
     requires f_listen_for_new_imported_blocks.requires(process, block)
     requires process' == f_listen_for_new_imported_blocks(process, block).state    
-    requires inv5_body(process)
+    requires inv_queued_att_duty_is_rcvd_duty_body(process)
     requires inv_strictly_increasing_queue_of_att_duties_body(process)
     requires inv_queued_att_duty_is_higher_than_latest_served_att_duty_body(process)
     ensures inv_queued_att_duty_is_higher_than_latest_served_att_duty_body(process')
@@ -2002,7 +2002,7 @@ module Fnc_Invs_1_26
                     rcvd_attestation_shares := process.rcvd_attestation_shares - att_consensus_instances_already_decided.Keys                    
                 );    
 
-        assert inv5_body(process);
+        assert inv_queued_att_duty_is_rcvd_duty_body(process);
         assert inv_strictly_increasing_queue_of_att_duties_body(process);
         assert inv_queued_att_duty_is_higher_than_latest_served_att_duty_body(process);
                     
@@ -2020,7 +2020,7 @@ module Fnc_Invs_1_26
                 )                
             );
 
-            assert inv5_body(process);
+            assert inv_queued_att_duty_is_rcvd_duty_body(process);
             assert inv_strictly_increasing_queue_of_att_duties_body(process);
             assert inv_queued_att_duty_is_higher_than_latest_served_att_duty_body(process);
 
@@ -2040,7 +2040,7 @@ module Fnc_Invs_1_26
     )
     requires f_att_consensus_decided.requires(process, id, decided_attestation_data)
     requires process' == f_att_consensus_decided(process, id, decided_attestation_data).state     
-    requires inv5_body(process)
+    requires inv_queued_att_duty_is_rcvd_duty_body(process)
     requires inv_strictly_increasing_queue_of_att_duties_body(process)
     requires inv_queued_att_duty_is_higher_than_latest_served_att_duty_body(process)
     ensures inv_queued_att_duty_is_higher_than_latest_served_att_duty_body(process')
@@ -2076,7 +2076,7 @@ module Fnc_Invs_1_26
                 )
             );
 
-        assert inv5_body(process);
+        assert inv_queued_att_duty_is_rcvd_duty_body(process);
         assert inv_strictly_increasing_queue_of_att_duties_body(process);
         assert inv_queued_att_duty_is_higher_than_latest_served_att_duty_body(process);
 
@@ -2442,7 +2442,7 @@ module Fnc_Invs_1_26
     )  
     requires f_serve_attestation_duty.requires(process, attestation_duty)
     requires process' == f_serve_attestation_duty(process, attestation_duty).state
-    requires inv5_body(process)
+    requires inv_queued_att_duty_is_rcvd_duty_body(process)
     requires inv_latest_served_duty_is_rcvd_duty_body(process)
     requires concl_future_att_duty_is_higher_than_rcvd_att_duty_body(process, attestation_duty)
     requires inv_strictly_increasing_queue_of_att_duties_body(process)
@@ -2456,7 +2456,7 @@ module Fnc_Invs_1_26
                 all_rcvd_duties := process.all_rcvd_duties + {attestation_duty}
             );        
 
-        assert inv5_body(process_mod);
+        assert inv_queued_att_duty_is_rcvd_duty_body(process_mod);
         assert inv_latest_served_duty_is_rcvd_duty_body(process_mod);
         assert inv_strictly_increasing_queue_of_att_duties_body(process_mod);                        
         assert inv_queued_att_duty_is_higher_than_latest_served_att_duty_body(process_mod);         
@@ -2640,7 +2640,7 @@ module Fnc_Invs_1_26
     )
     requires f_check_for_next_queued_duty.requires(process)
     requires process' == f_check_for_next_queued_duty(process).state    
-    requires inv5_body(process)
+    requires inv_queued_att_duty_is_rcvd_duty_body(process)
     requires inv_consensus_instance_only_for_slot_in_which_dvc_has_rcvd_att_duty_body(process)
     ensures inv_consensus_instance_only_for_slot_in_which_dvc_has_rcvd_att_duty_body(process')
     decreases process.attestation_duties_queue
@@ -2664,7 +2664,7 @@ module Fnc_Invs_1_26
                             new_attestation_slashing_db
                         )                        
                     );
-                    assert inv5_body(process_mod);
+                    assert inv_queued_att_duty_is_rcvd_duty_body(process_mod);
                     lemma_inv_consensus_instance_only_for_slot_in_which_dvc_has_rcvd_att_duty_f_check_for_next_queued_duty(process_mod, process');
                 }
                 else
@@ -2691,7 +2691,7 @@ module Fnc_Invs_1_26
     )
     requires f_att_consensus_decided.requires(process, id, decided_attestation_data)
     requires process' == f_att_consensus_decided(process, id, decided_attestation_data).state         
-    requires inv5_body(process)
+    requires inv_queued_att_duty_is_rcvd_duty_body(process)
     requires inv_consensus_instance_only_for_slot_in_which_dvc_has_rcvd_att_duty_body(process)
     ensures inv_consensus_instance_only_for_slot_in_which_dvc_has_rcvd_att_duty_body(process')
     {
@@ -2726,12 +2726,12 @@ module Fnc_Invs_1_26
                 )
             );
 
-        assert inv5_body(process);
+        assert inv_queued_att_duty_is_rcvd_duty_body(process);
         assert inv_consensus_instance_only_for_slot_in_which_dvc_has_rcvd_att_duty_body(process);
 
         var ret_dvc := f_check_for_next_queued_duty(process).state;
-        lemma_inv5_f_check_for_next_queued_duty(process, ret_dvc);
-        assert inv5_body(ret_dvc);
+        lemma_inv_queued_att_duty_is_rcvd_duty_f_check_for_next_queued_duty(process, ret_dvc);
+        assert inv_queued_att_duty_is_rcvd_duty_body(ret_dvc);
         
         lemma_inv_consensus_instance_only_for_slot_in_which_dvc_has_rcvd_att_duty_f_check_for_next_queued_duty(process, ret_dvc);
         assert inv_consensus_instance_only_for_slot_in_which_dvc_has_rcvd_att_duty_body(ret_dvc);
@@ -2746,7 +2746,7 @@ module Fnc_Invs_1_26
     )  
     requires f_serve_attestation_duty.requires(process, attestation_duty)
     requires process' == f_serve_attestation_duty(process, attestation_duty).state
-    requires inv5_body(process)
+    requires inv_queued_att_duty_is_rcvd_duty_body(process)
     requires inv_consensus_instance_only_for_slot_in_which_dvc_has_rcvd_att_duty_body(process)
     ensures inv_consensus_instance_only_for_slot_in_which_dvc_has_rcvd_att_duty_body(process')
     {
@@ -2755,7 +2755,7 @@ module Fnc_Invs_1_26
                 all_rcvd_duties := process.all_rcvd_duties + {attestation_duty}
             );        
 
-        assert inv5_body(process_mod);
+        assert inv_queued_att_duty_is_rcvd_duty_body(process_mod);
         assert inv_consensus_instance_only_for_slot_in_which_dvc_has_rcvd_att_duty_body(process_mod);
         
         lemma_inv_consensus_instance_only_for_slot_in_which_dvc_has_rcvd_att_duty_f_check_for_next_queued_duty(process_mod, process');        
@@ -2768,7 +2768,7 @@ module Fnc_Invs_1_26
     )
     requires f_listen_for_new_imported_blocks.requires(process, block)
     requires process' == f_listen_for_new_imported_blocks(process, block).state        
-    requires inv5_body(process)
+    requires inv_queued_att_duty_is_rcvd_duty_body(process)
     requires inv_consensus_instance_only_for_slot_in_which_dvc_has_rcvd_att_duty_body(process)
     ensures inv_consensus_instance_only_for_slot_in_which_dvc_has_rcvd_att_duty_body(process')
     {
@@ -2790,7 +2790,7 @@ module Fnc_Invs_1_26
                     rcvd_attestation_shares := process.rcvd_attestation_shares - att_consensus_instances_already_decided.Keys                    
                 );    
         
-        assert inv5_body(process);
+        assert inv_queued_att_duty_is_rcvd_duty_body(process);
         assert inv_consensus_instance_only_for_slot_in_which_dvc_has_rcvd_att_duty_body(process);
 
         if process.current_attestation_duty.isPresent() && process.current_attestation_duty.safe_get().slot in att_consensus_instances_already_decided
@@ -2806,7 +2806,7 @@ module Fnc_Invs_1_26
                 )                
             );
             
-            assert inv5_body(process);
+            assert inv_queued_att_duty_is_rcvd_duty_body(process);
             assert inv_consensus_instance_only_for_slot_in_which_dvc_has_rcvd_att_duty_body(process);
 
             lemma_inv_consensus_instance_only_for_slot_in_which_dvc_has_rcvd_att_duty_f_check_for_next_queued_duty(process, process');
@@ -2862,7 +2862,7 @@ module Fnc_Invs_1_26
     )
     requires f_check_for_next_queued_duty.requires(process)
     requires process' == f_check_for_next_queued_duty(process).state    
-    requires inv5_body(process)
+    requires inv_queued_att_duty_is_rcvd_duty_body(process)
     requires inv_consensus_instances_only_for_rcvd_duties_body(process)
     ensures inv_consensus_instances_only_for_rcvd_duties_body(process')
     decreases process.attestation_duties_queue
@@ -2886,7 +2886,7 @@ module Fnc_Invs_1_26
                             new_attestation_slashing_db
                         )                        
                     );
-                    assert inv5_body(process_mod);
+                    assert inv_queued_att_duty_is_rcvd_duty_body(process_mod);
                     lemma_inv_consensus_instances_only_for_rcvd_duties_f_check_for_next_queued_duty(process_mod, process');
                 }
                 else
@@ -2913,7 +2913,7 @@ module Fnc_Invs_1_26
     )
     requires f_att_consensus_decided.requires(process, id, decided_attestation_data)
     requires process' == f_att_consensus_decided(process, id, decided_attestation_data).state         
-    requires inv5_body(process)
+    requires inv_queued_att_duty_is_rcvd_duty_body(process)
     requires inv_consensus_instances_only_for_rcvd_duties_body(process)
     ensures inv_consensus_instances_only_for_rcvd_duties_body(process')
     {
@@ -2948,12 +2948,12 @@ module Fnc_Invs_1_26
                 )
             );
 
-        assert inv5_body(process);
+        assert inv_queued_att_duty_is_rcvd_duty_body(process);
         assert inv_consensus_instances_only_for_rcvd_duties_body(process);
 
         var ret_dvc := f_check_for_next_queued_duty(process).state;
-        lemma_inv5_f_check_for_next_queued_duty(process, ret_dvc);
-        assert inv5_body(ret_dvc);
+        lemma_inv_queued_att_duty_is_rcvd_duty_f_check_for_next_queued_duty(process, ret_dvc);
+        assert inv_queued_att_duty_is_rcvd_duty_body(ret_dvc);
         
         lemma_inv_consensus_instances_only_for_rcvd_duties_f_check_for_next_queued_duty(process, ret_dvc);
         assert inv_consensus_instances_only_for_rcvd_duties_body(ret_dvc);
@@ -2968,7 +2968,7 @@ module Fnc_Invs_1_26
     )  
     requires f_serve_attestation_duty.requires(process, attestation_duty)
     requires process' == f_serve_attestation_duty(process, attestation_duty).state
-    requires inv5_body(process)
+    requires inv_queued_att_duty_is_rcvd_duty_body(process)
     requires inv_consensus_instances_only_for_rcvd_duties_body(process)
     ensures inv_consensus_instances_only_for_rcvd_duties_body(process')
     {
@@ -2977,7 +2977,7 @@ module Fnc_Invs_1_26
                 all_rcvd_duties := process.all_rcvd_duties + {attestation_duty}
             );        
 
-        assert inv5_body(process_mod);
+        assert inv_queued_att_duty_is_rcvd_duty_body(process_mod);
         assert inv_consensus_instances_only_for_rcvd_duties_body(process_mod);
         
         lemma_inv_consensus_instances_only_for_rcvd_duties_f_check_for_next_queued_duty(process_mod, process');        
@@ -2990,7 +2990,7 @@ module Fnc_Invs_1_26
     )
     requires f_listen_for_new_imported_blocks.requires(process, block)
     requires process' == f_listen_for_new_imported_blocks(process, block).state        
-    requires inv5_body(process)
+    requires inv_queued_att_duty_is_rcvd_duty_body(process)
     requires inv_consensus_instances_only_for_rcvd_duties_body(process)
     ensures inv_consensus_instances_only_for_rcvd_duties_body(process')
     {
@@ -3012,7 +3012,7 @@ module Fnc_Invs_1_26
                     rcvd_attestation_shares := process.rcvd_attestation_shares - att_consensus_instances_already_decided.Keys                    
                 );    
         
-        assert inv5_body(process);
+        assert inv_queued_att_duty_is_rcvd_duty_body(process);
         assert inv_consensus_instances_only_for_rcvd_duties_body(process);
 
         if process.current_attestation_duty.isPresent() && process.current_attestation_duty.safe_get().slot in att_consensus_instances_already_decided
@@ -3028,7 +3028,7 @@ module Fnc_Invs_1_26
                 )                
             );
             
-            assert inv5_body(process);
+            assert inv_queued_att_duty_is_rcvd_duty_body(process);
             assert inv_consensus_instances_only_for_rcvd_duties_body(process);
 
             lemma_inv_consensus_instances_only_for_rcvd_duties_f_check_for_next_queued_duty(process, process');
